papers/116_stefan_rass/L0.thy
@@ -15,7 +15,9 @@ begin
 text\<open>\<open>L\<^sub>D\<close>, defined as part of the proof for the Time Hierarchy Theorem.
 
   "The “diagonal-language” \<open>L\<^sub>D\<close> is thus defined over the alphabet \<open>\<Sigma> = {0, 1}\<close> as
-      \<open>LD := {w \<in> \<Sigma>\<^sup>*: M\<^sub>w halts and rejects w within \<le> T(len (w)) steps}\<close>.    (9)"\<close>
+       \<open>LD := {w \<in> \<Sigma>\<^sup>*: M\<^sub>w halts and rejects w within \<le> T(len(w)) steps}\<close>.    (9)"\<close>
+
+(* this is incorrect as it still depends on the whole \<open>w\<close> and not just the portion *)
 
 definition L\<^sub>D :: "lang"
   where LD_def[simp]: "L\<^sub>D \<equiv> {w. let M\<^sub>w = TM_decode_pad w in
@@ -46,6 +48,9 @@ lemma tht_h1: "DTIME t \<subseteq> DTIME T" sorry
 
 lemma tht_h2: "L\<^sub>D \<in> DTIME T" "L\<^sub>D \<notin> DTIME t" sorry
 
+(* this formulation is used in Hopcroft's Thm. 12.9 *)
+lemma tht_h2': "L\<^sub>D \<in> DTIME T - DTIME t" oops
+
 theorem time_hierarchy: "DTIME t \<subset> DTIME T"
 proof
   show "DTIME t \<subseteq> DTIME T" by (rule tht_h1)
@@ -53,18 +58,59 @@ proof
   then show "DTIME t \<noteq> DTIME T" by blast
 qed
 
+end \<comment> \<open>\<^locale>\<open>tht_assms\<close>\<close>
 
-section\<open>L\<^sub>0\<close>
+
+section\<open>\<open>L\<^sub>0\<close>\<close>
+
+text\<open>From the proof of Lemma 4.6, p14:
+
+   "To retain \<open>L\<^sub>D \<inter> SQ \<in> DTIME(T)\<close>, we must choose \<open>T\<close> so large that the decision
+    \<open>w \<in> SQ\<close> is possible within the time limit incurred by \<open>T\<close>, so we add \<open>T(n) \<ge> n\<^sup>3\<close>
+    to our hypothesis besides Assumption 4.4 (note that we do not need an optimal
+    complexity bound here)."\<close>
+
+locale tht_sq_assms = tht_assms +
+  assumes "T n \<ge> n^3"
+begin
 
 definition L\<^sub>0 :: lang
   where L0_def[simp]: "L\<^sub>0 \<equiv> L\<^sub>D \<inter> SQ"
 
 
+lemma L\<^sub>D_adj_sq_iff:
+  fixes w
+  defines "w' \<equiv> gn_inv (adj_square (gn w))"
+  shows "w \<in> L\<^sub>D \<longleftrightarrow> w' \<in> L\<^sub>D"
+    \<comment> \<open>Idea: since \<open>n\<close> and \<open>adj_square n\<close> share their prefix (@{thm adj_sq_shared_prefix_log}),
+  the relevant parts are identical and this lemma should hold.
+
+  Note: with the current definition of \<^const>\<open>L\<^sub>D\<close>, this likely does not hold,
+        as the whole word \<open>w\<close> is referenced in the definition.\<close>
+
+  thm adj_sq_shared_prefix_log
+  sorry
+
+lemma L\<^sub>D_L\<^sub>0_adj_sq_iff:
+  fixes w
+  defines "w' \<equiv> gn_inv (adj_square (gn w))"
+  shows "w \<in> L\<^sub>D \<longleftrightarrow> w' \<in> L\<^sub>0"
+proof
+  assume "w \<in> L\<^sub>D"
+  then have "w' \<in> L\<^sub>D" unfolding w'_def by (fold L\<^sub>D_adj_sq_iff)
+  moreover have "w' \<in> SQ" unfolding w'_def SQ_def
+    using adj_sq_correct and adj_sq_gt_0 by (intro CollectI) (subst inv_gn_id)
+  ultimately show "w' \<in> L\<^sub>0" unfolding L0_def ..
+next
+  assume "w' \<in> L\<^sub>0"
+  then have "w' \<in> L\<^sub>D" unfolding L0_def ..
+  then show "w \<in> L\<^sub>D" unfolding w'_def by (fold L\<^sub>D_adj_sq_iff)
+qed
 
 (* Lemma 4.6, p15 *)
 theorem dens_L0: "dens L\<^sub>0 n \<le> dsqrt n" oops
 
 
-end (* locale *)
+end \<comment> \<open>\<^locale>\<open>tht_sq_assms\<close>\<close>
 
 end
