papers/116_stefan_rass/Language_Density.thy
@@ -4,6 +4,9 @@ begin
 
 type_synonym lang = "word set"
 
+\<comment> \<open>The empty word.\<close>
+abbreviation \<epsilon> :: word where "\<epsilon> \<equiv> []"
+
 
 section\<open>Language Density\<close>
 
